src/opt/Simulation.v
@@ -32,6 +32,25 @@ Module Simulation.
       exists src1,
         <<INTERNAL: Configuration.internal_steps src0 src1>> /\
         <<TERM: Configuration.is_terminal src1>>.
+  End Simulation.
+
+  Structure t (prog_src prog_tgt:Configuration.syntax): Prop := mk {
+    sim: forall (src tgt:Configuration.t), Prop;
+    init: INIT prog_src prog_tgt sim;
+    step: STEP sim;
+    terminal: TERMINAL sim;
+  }.
+
+  Section BaseSimulation.
+    Variable (prog_src prog_tgt:Configuration.syntax).
+    Variable (sim: forall (src tgt:Configuration.t), Prop).
+
+    Inductive sim_lift (src tgt:Configuration.t): Prop :=
+    | sim_lift_intro
+        (SIM: sim src tgt)
+        (SRC: Configuration.feasible src)
+        (TGT: Configuration.feasible tgt)
+    .
 
     Definition FEASIBLE: Prop :=
       forall src tgt
@@ -43,13 +62,9 @@ Module Simulation.
       forall src0 tgt0 reading tgt2
         (SIM: sim src0 tgt0)
         (STEP: Configuration.base_step tgt0 reading tgt2)
-        (VALIDATION:
-           forall (READING: reading),
-           exists src0' tgt0',
-             <<SRC: Configuration.internal_steps src0 src0'>> /\
-             <<TGT: Configuration.internal_steps tgt0 tgt0'>> /\
-             <<CONFIRM: ~ Messages.declared tgt0'.(Configuration.messages)>> /\
-             <<SIM: sim src0' tgt0'>>),
+        (SRC0: reading -> Configuration.feasible src0)
+        (TGT0: Configuration.feasible tgt0)
+        (TGT2: Configuration.feasible tgt2),
       exists src1 src2,
         <<INTERNAL: Configuration.internal_steps src0 src1>> /\
         <<STEP: Configuration.internal_step src1 src2>> /\
@@ -58,72 +73,73 @@ Module Simulation.
     Definition EXTERNAL_STEP: Prop :=
       forall src0 tgt0 e tgt2
         (SIM: sim src0 tgt0)
-        (STEP: Configuration.external_step tgt0 e tgt2),
+        (STEP: Configuration.external_step tgt0 e tgt2)
+        (SRC0: Configuration.feasible src0)
+        (TGT0: Configuration.feasible tgt0)
+        (TGT2: Configuration.feasible tgt2),
       exists src1 src2,
         <<INTERNAL: Configuration.internal_steps src0 src1>> /\
         <<STEP: Configuration.external_step src1 e src2>> /\
         <<SIM: sim src2 tgt2>>.
 
-    Lemma internal_step (B:BASE_STEP):
+    Lemma internal_step (F:FEASIBLE) (B:BASE_STEP):
       forall src0 tgt0 tgt2
         (SIM: sim src0 tgt0)
-        (STEP: Configuration.internal_step tgt0 tgt2),
+        (STEP: Configuration.internal_step tgt0 tgt2)
+        (TGT2: Configuration.feasible tgt2),
       exists src1 src2,
         <<INTERNAL: Configuration.internal_steps src0 src1>> /\
         <<STEP: Configuration.internal_step src1 src2>> /\
         <<SIM: sim src2 tgt2>>
-    with internal_steps (B:BASE_STEP):
-      forall src0 tgt0 tgt1
+    with feasible (F:FEASIBLE) (B:BASE_STEP):
+      forall src0 tgt0
         (SIM: sim src0 tgt0)
-        (STEP: Configuration.internal_steps tgt0 tgt1),
-      exists src1,
-        <<INTERNAL: Configuration.internal_steps src0 src1>> /\
-        <<SIM: sim src1 tgt1>>.
+        (TGT0: Configuration.feasible tgt0),
+        Configuration.feasible src0.
     Proof.
       - i. inv STEP0; eapply B; eauto.
-        + congruence.
-        + exploit internal_steps; eauto. i. des.
-          eexists _, _. splits; eauto.
-      - i. revert src0 SIM. induction STEP0.
-        + i. eexists. splits; eauto.
-          econs 1.
-        + i. exploit internal_step; eauto. i. des.
-          exploit IHSTEP0; eauto. i. des.
-          eexists. splits; [|eauto].
-          eapply Configuration.internal_steps_append; eauto.
-          econs 2; eauto.
+        eapply Configuration.internal_steps_feasible; eauto.
+        econs 2; eauto.
+        + econs 1. eauto.
+        + econs 1.
+      - i. inv TGT0. revert src0 SIM CONFIRM. induction STEPS.
+        + i. eapply F; eauto.
+        + i. exploit internal_step; eauto.
+          { econs; eauto. }
+          i. des.
+          exploit IHSTEPS; eauto. i. des.
+          eapply Configuration.internal_steps_feasible; eauto.
+          eapply Configuration.internal_steps_feasible; eauto.
+          econs 2; eauto. econs 1.
     Qed.
 
-    Lemma feasible_lemma (F:FEASIBLE) (B:BASE_STEP)
-          src tgt
-          (SIM: sim src tgt)
-          (FEASIBLE: Configuration.feasible tgt):
-      Configuration.feasible src.
+    Lemma step_lemma (F:FEASIBLE) (B:BASE_STEP) (E:EXTERNAL_STEP): STEP (sim_lift).
     Proof.
-      inv FEASIBLE. exploit internal_steps; eauto. i. des.
-      exploit F; eauto. intro X. inv X.
-      econs; [|eauto].
-      eapply Configuration.internal_steps_append; eauto.
-    Qed.
-
-    Lemma step_lemma (F:FEASIBLE) (B:BASE_STEP) (E:EXTERNAL_STEP): STEP.
-    Proof.
-      ii. inv STEP0.
+      ii. inv SIM. inv STEP0.
       - exploit internal_step; eauto. i. des.
+        exploit feasible; eauto. intro SRC2.
         eexists _, _. splits; eauto.
-        econs; eauto.
-        eapply feasible_lemma; eauto.
+        + econs; eauto.
+        + econs; eauto.
       - exploit E; eauto. i. des.
+        exploit feasible; eauto. intro SRC2.
         eexists _, _. splits; eauto.
-        econs; eauto.
-        eapply feasible_lemma; eauto.
+        + econs; eauto.
+        + econs; eauto.
     Qed.
-  End Simulation.
 
-  Structure t (prog_src prog_tgt:Configuration.syntax) := mk {
-    sim: forall (src tgt:Configuration.t), Prop;
-    init: INIT prog_src prog_tgt sim;
-    step: STEP sim;
-    terminal: TERMINAL sim;
-  }.
+    Lemma sim_lemma
+          src tgt
+          (I:INIT src tgt sim)
+          (F:FEASIBLE) (B:BASE_STEP) (E:EXTERNAL_STEP)
+          (T:TERMINAL sim):
+      Simulation.t src tgt.
+    Proof.
+      econs; try apply step_lemma; auto.
+      - econs; auto.
+        + apply Configuration.init_feasible.
+        + apply Configuration.init_feasible.
+      - ii. inv SIM. exploit T; eauto.
+    Qed.
+  End BaseSimulation.
 End Simulation.
